src/KInduction_example.v
@@ -29,10 +29,7 @@ Proof.
   unfold safety_nth_offset.
   unfold safety_nth_conj.
   unfold prop_nth_init_conj.
-  unfold loop_free.
   unfold path.
-  unfold no_loop.
-  unfold no_loop'.
   unfold sseq.
   unfold nth.
   unfold state.
@@ -59,7 +56,7 @@ Qed.
 Goal k_induction_post_conj ex2_I ex2_T ex2_P 2.
 Proof.
   unfold ex2_I, ex2_T, ex2_P.
-  unfold k_induction_post_conj, k_ind_step_conj, safety_nth_offset, safety_nth_conj, prop_nth_init_conj, loop_free, path, no_loop, no_loop', sseq, nth, state.
+  unfold k_induction_post_conj, k_ind_step_conj, safety_nth_offset, safety_nth_conj, prop_nth_init_conj, path, sseq, nth, state.
   repeat rewrite -> Nat.add_0_l;
   repeat rewrite -> Nat.add_0_r.
   split.
@@ -70,7 +67,7 @@ Qed.
 Goal k_induction_post_conj ex3_I ex3_T ex3_P 5.
 Proof.
   unfold ex3_I, ex3_T, ex3_P.
-  unfold k_induction_post_conj, k_ind_step_conj, safety_nth_offset, safety_nth_conj, prop_nth_init_conj, loop_free, path, no_loop, no_loop', sseq, nth, state.
+  unfold k_induction_post_conj, k_ind_step_conj, safety_nth_offset, safety_nth_conj, prop_nth_init_conj, path, sseq, nth, state.
   repeat rewrite -> Nat.add_0_l;
   repeat rewrite -> Nat.add_0_r.
   split.
